\begin{exer}[4.1]
    $ $
    \begin{enumerate}[label=(\alph*)]
        \item
            \todo[inline,caption={}]{
                Proofread!
            }
            This proof is rather complicated since we use stepwise induction inside another stepwise induction proof.
            Let $G_u[v]$ be defined to be the formula $\flatlist(u) \land \flatlist(v) \rightarrow \flatlist(\concat(u, v))$.
            Let $F[u]$ be defined to be the formula $\forall v.\, G_u[v]$.
            We prove by stepwise induction on $u$ that $F[u]$.

            \begin{itemize}
                \item
                    For the base case, we consider arbitrary $\atom u$ and prove $F[u]$.
                    In other words, we want to show that $\forall v.\, G_u[v]$.
                    \begin{itemize}
                        \item
                            For the base case, we consider arbitrary $\atom v$ and prove $G_u[v]$.
                            In other words, we want to prove $\flatlist(u) \land \flatlist(v) \rightarrow \flatlist(\concat(u, v))$.
                            Since $\atom u$ and $\atom v$, $\flatlist(\concat(u, v)) = \flatlist(\cons(u, v)) \leftrightarrow \atom(u) \land \flatlist(v) = \true$ by \textsf{(concat atom)}, \textsf{(flat atom)}, \textsf{(flat list)}.
                        \item
                            Assume as the inductive hypothesis that for arbitrary list $y$, $G_u[y]$.
                            Let $x$ be given.
                            We want to show that $G_u[\cons(x, y)]$.
                            In other words, we want to show that $\flatlist(u) \land \flatlist(\cons(x, y)) \rightarrow \flatlist(\concat(u, \cons(x, y)))$.
                            \begin{align*}
                                &\flatlist(u) \land \flatlist(\cons(x, y)) \\
                                &\quad\leftrightarrow \atom(u) \land \flatlist(\cons(x, y)) & (\atom(u)) \\
                                &\quad\leftrightarrow \flatlist(\cons(u, \cons(x, y))) & \textsf{(flat list)} \\
                                &\quad\leftrightarrow \flatlist(\concat(u, \cons(x, y))) & \textsf{(concat atom)} \\
                            \end{align*}
                            Therefore, the inductive step has been shown.
                    \end{itemize}
                    By stepwise induction, we have shown that $\forall v.\, G_u[v]$.
                \item
                    Assume as the inductive hypothesis that $F[y]$ for arbitrary $y$.
                    In other words, we are assuming that $\forall v.\, G_y[v]$, which is equivalent to $\forall v.\, \flatlist(y) \land \flatlist(v) \rightarrow \flatlist(\concat(y, v))$.
                    Let $x$ be given.
                    We want to show that $F[\cons(x, y)]$.
                    In other words, $\forall v.\, G_{\cons(x, y)}[v]$, which is equivalent to $\forall v.\, \flatlist(\cons(x, y)) \land \flatlist(v) \rightarrow \flatlist(\concat(\cons(x, y), v))$.
                    We will first examine the hypothesis:
                    \begin{align*}
                        & \flatlist(\cons(x, y)) \land \flatlist(v) \\
                        & \leftrightarrow \atom x \land \flatlist(y) \land \flatlist(v) & \textsf{(flat list)} \\
                    \end{align*}
                    Therefore, if $\neg\atom x$, we are done.
                    Suppose $\atom x$.
                    \begin{align*}
                        & \atom x \land \flatlist(y) \land \flatlist(v) \\
                        & \leftrightarrow \flatlist(y) \land \flatlist(v) \\
                        & \rightarrow \flatlist(\concat(y, v)) & \text{(inductive hypothesis)} \\
                        & \leftrightarrow \flatlist(\cons(x, \concat(y, v))) & \textsf{(flat list)} \\
                        & = \flatlist(\concat(\cons(x, y), v)) & \textsf{(concat list)} \\
                    \end{align*}
            \end{itemize}
            Therefore, we have shown that $\forall u.\, F[u]$.
        \item
            Let $F[u]: \flatlist(u) \rightarrow \flatlist(\revlist(u))$.
            We will show that $F[u]$ is true for any $u$ by stepwise induction on $u$.
            For the base case, we consider arbitrary $\atom u$ and prove $F[u]$.
            This is trivial by \textsf{(reverse atom)} and \textsf{(flat atom)}.
            Assume as the inductive hypothesis that for arbtrary list $v$, $F[v]$ is true.
            We want to prove that, for arbitrary list $u$, $F[\cons(u, v)]$.
            Suppose that $\atom u$
            \begin{align*}
                \flatlist(\cons(u, v))
                    &\leftrightarrow \atom(u) \land \flatlist(v) & \textsf{(flat list)}\\
                    &\rightarrow \atom(u) \land \flatlist(\revlist(v)) & \text{(inductive hypothesis)}\\
                    &\leftrightarrow \flatlist(\cons(u, \revlist(v))) & \textsf{(flat list)} \\
                    &= \flatlist(\concat(u, \revlist(v))) & \textsf{(concat atom)} \\
                    &= \flatlist(\concat(\revlist(u), \revlist(v))) & \textsf{(reverse atom)} \\
                    &= \flatlist(\revlist(\concat(u, v))) & \textsf{(reverse list)} \\
            \end{align*}
            Thus $\flatlist(\cons(u, v)) \rightarrow \flatlist(\revlist(\concat(u, v)))$.
            Suppose that $\neg\atom u$.
            Then
            \begin{align*}
                \flatlist(\cons(u, v)) \leftrightarrow \atom(u) \land \flatlist(v)
            \end{align*}
            by $\textsf{(flat list)}$, but $\atom(u)$ is false, so we are done.
            Thus we have shown that $F[u]$ is true for any arbitrary $u$.
    \end{enumerate}
\end{exer}
